chapter07/exercises/library.dfy
@@ -1,0 +1,47 @@
+module Library {
+  function DropLast<T>(theSeq: seq<T>) : seq<T>
+    requires 0 < |theSeq|
+  {
+    theSeq[..|theSeq|-1]
+  }
+
+  function Last<T>(theSeq: seq<T>) : T
+    requires 0 < |theSeq|
+  {
+    theSeq[|theSeq|-1]
+  }
+
+  function UnionSeqOfSets<T>(theSets: seq<set<T>>) : set<T>
+  {
+    if |theSets| == 0 then {} else
+      UnionSeqOfSets(DropLast(theSets)) + Last(theSets)
+  }
+
+  // As you can see, Dafny's recursion heuristics easily complete the recursion
+  // induction proofs, so these two statements could easily be ensures of
+  // UnionSeqOfSets. However, the quantifiers combine with native map axioms
+  // to be a bit trigger-happy, so we've pulled them into independent lemmas
+  // you can invoke only when needed.
+  lemma SetsAreSubsetsOfUnion<T>(theSets: seq<set<T>>)
+    ensures forall idx | 0<=idx<|theSets| :: theSets[idx] <= UnionSeqOfSets(theSets)
+  {
+  }
+
+  lemma EachUnionMemberBelongsToASet<T>(theSets: seq<set<T>>)
+    ensures forall member | member in UnionSeqOfSets(theSets) ::
+          exists idx :: 0<=idx<|theSets| && member in theSets[idx]
+  {
+  }
+
+  // Convenience function for learning a particular index (invoking Hilbert's
+  // Choose on the exists in EachUnionMemberBelongsToASet).
+  lemma GetIndexForMember<T>(theSets: seq<set<T>>, member: T) returns (idx:int)
+    requires member in UnionSeqOfSets(theSets)
+    ensures 0<=idx<|theSets|
+    ensures member in theSets[idx]
+  {
+    EachUnionMemberBelongsToASet(theSets);
+    var chosenIdx :| 0<=chosenIdx<|theSets| && member in theSets[chosenIdx];
+    idx := chosenIdx;
+  }
+}
